code/salsa-family/Hacl.Impl.Chacha20.fst
@@ -17,6 +17,7 @@ module Spec = Spec.Chacha20
 type state = lbuffer uint32 16
 type idx = n:size_t{v n < 16}
 
+
 inline_for_extraction
 let v = size_v
 inline_for_extraction
@@ -111,19 +112,17 @@ private
 val chacha20_core:
   k:state ->
   st:state ->
-  ctr:size_t ->
   Stack unit
     (requires (fun h -> live h k /\ live h st /\ disjoint st k))
-    (ensures  (fun h0 _ h1 -> preserves_live h0 h1 /\ modifies2 st k h0 h1 /\
-			  (let s = as_lseq st h0 in
-			   let s = Spec.Lib.IntSeq.(s.[12] <- size_to_uint32 ctr) in
-			   as_lseq k h1 == Spec.chacha20_core s)))
+    (ensures  (fun h0 _ h1 -> preserves_live h0 h1 /\ modifies1 k h0 h1 /\
+		as_lseq k h1 == Spec.chacha20_core (as_lseq st h0)))
+#reset-options "--z3rlimit 50"
 [@ "c_inline"]
-let chacha20_core k st ctr =
-  st.(index 12) <- size_to_uint32 ctr;
+let chacha20_core k st =
   copy (size 16) st k;
   rounds k;
-  map2 (size 16) (fun x y -> add_mod #U32 x y) k st
+  map2 (size 16) (add_mod #U32) k st;
+  ()
 
 [@ "c_inline"]
 val setup:
@@ -140,14 +139,14 @@ val setup:
 #reset-options "--z3rlimit 50 --max_fuel 0"
 [@ "c_inline"]
 let setup st k n =
-  st.(0) <- u32 Spec.c0;
-  st.(1) <- u32 Spec.c1;
-  st.(2) <- u32 Spec.c2;
-  st.(3) <- u32 Spec.c3;
-  let st_k = sub st 4 8 in
-  uint32s_from_bytes_le #8 st_k k;
-  let st_n = sub st 13 3 in
-  uint32s_from_bytes_le #3 st_n n 
+  st.(index 0) <- u32 Spec.c0;
+  st.(index 1) <- u32 Spec.c1;
+  st.(index 2) <- u32 Spec.c2;
+  st.(index 3) <- u32 Spec.c3;
+  let st_k = sub st (index 4) (index 8) in
+  uint32s_from_bytes_le #8 (size 8) st_k k;
+  let st_n = sub st (index 13) (index 3) in
+  uint32s_from_bytes_le #3 (size 3) st_n n 
 
 (*
 [@ "c_inline"]
