specs/lib/fst/Spec.Lib.RawIntTypes.fst
@@ -18,6 +18,7 @@ let u64_from_UInt64 x = x
 let u128_from_UInt128 x = x
 
 let size_from_UInt32 x =  x
+
 let u8_to_UInt8 x = x
 
 let u16_to_UInt16 x = x
